changed the representation of Fix in L4a,L5, L5a
Not using the projection based representation of mutual fixpoints.
Now, there are separate bound variables for each member in a mutual fixpoint block.
Had to update the CPS translation and its tricky correctness proof.
The bodies of Fix, which must be lambdas, are now translated using the value translation (cps_cvt_val).
The replacement of the projection rule in eval_c is:

| eval_FixApp_c : forall lbt i k arg v bt,
    let len := Datatypes.length lbt in
    let pinds := seq 0 len in
    let sub := map (Fix_c' lbt) pinds in
    select i lbt = Some bt ->
    eval_c (Call_c (apply_bterm bt sub) k arg) v ->
    eval_c (Call_c (Fix_c' lbt i) k arg) v.

Now, these languages (L4a-L5a) are similar to the rest in terms of how fix is represented.
The proof of L4 to L4a correctness and L5a to L6 should be easier now.

Fixed the (L4) files broken due to broken imports due to the namespaces changes in Zoe's r7636, and added them back in _Coqproject
Everything (in the _CoqProject(s)) compiles on my machine when I do make clean; make -j8 -k at the root of the repo.

certicoq/theories/L4_deBruijn/L4a_to_L5.v
@@ -48,10 +48,51 @@ Open Scope nat_scope.
 
 (* MOVE to [SquiggleEq] *)
 
+Section GetOpid.
+Context {NVar Opid : Type}.
+
+Definition getOpid (n: @NTerm NVar Opid) : option Opid :=
+match n with
+| vterm _ => None
+| oterm o _ => Some o
+end. 
+Context {VarClass:Type} `{Deq NVar} `{VarType NVar VarClass}.
+
+Global Instance alphaGetOpid : Proper ((@alpha_eq NVar _ _ _ Opid) ==> eq) getOpid.
+Proof.
+  intros ? ? Hal.
+  inverts Hal; refl.
+Qed.
+
+End GetOpid.
 
 Instance NEqDec : Deq N.
 Proof using.
   intros x y. exists (N.eqb x y). apply N.eqb_eq.
+Defined.
+
+Definition deqOption {A:Type} `{Deq A} (oa ob : option A) : bool :=
+match (oa,ob) with
+| (Some a, Some b) => decide (a=b)
+| (None, None) => true
+| _ => false 
+end.
+
+Lemma deqOptionCorr {A:Type} `{Deq A} :
+  forall x y, deqOption x y = true <-> x = y.
+Proof.
+  destruct x, y; unfold deqOption; simpl; auto; 
+  unfold decide; try rewrite  Decidable_spec;
+  split; intro;
+  subst; try discriminate; auto.
+  inverts H0. refl.
+Qed.
+
+
+
+Instance optionEqDec {A:Type} `{Deq A}: Deq (option A).
+Proof using.
+  intros x y. exists (deqOption x y). apply deqOptionCorr.
 Defined.
 
 Require Import Common.classes Common.AstCommon.
@@ -83,10 +124,13 @@ Definition dcon : Set := inductive * N.
 
 Inductive L4Opid : Set :=
  | NLambda
- | NFix (nMut : nat) (** number of functions that are mutually defined*)
+(** number of functions that are mutually defined, index of the one which
+is referred to here.*)
+ | NFix (nMut index: nat) 
  | NDCon (dc : dcon) (nargs : nat)
  | NApply
- | NProj (selector :nat) (** which one to project out*)
+(* Not longer using projection based semantics for mutual fixpoints 
+| NProj (selector :nat) (** which one to project out*) *)
  | NLet
  | NMatch (dconAndNumArgs : list (dcon * nat)).
 
@@ -94,10 +138,10 @@ Inductive L4Opid : Set :=
 Definition OpBindingsL4 (nc : L4Opid) : list nat :=
   match nc with
   | NLambda    => [1]
-  | NFix nMut => repeat 1 nMut
+  | NFix nMut _ => repeat nMut nMut
   | NDCon _ nargs    => repeat 0 nargs
   | NApply     => [0,0]
-  | NProj _ => [0]
+(*  | NProj _ => [0] *)
   | NLet => [0,1]
   | NMatch numargsInBranches => 0::(List.map snd numargsInBranches)
   end.
@@ -124,12 +168,14 @@ Instance CoqL4GenericTermSig : GenericTermSig L4Opid:=
 Inductive L5Opid : Set :=
  | CLambda 
  | CKLambda
- | CFix (nMut : nat) (** number of functions that are mutually defined*)
+(** number of functions that are mutually defined, index of the one which
+is referred to here.*)
+ | CFix (nMut index : nat)
  | CDCon (dc : dcon) (nargs : nat)
  | CHalt 
  | CRet (** application of a continuation lambda ([CKLambda]) *)
  | CCall (** a bit like apply in source language *)
- | CProj (selector :nat) (** which one to project out*)
+(* | CProj (selector :nat) (** which one to project out*) *)
  (* nat may be ineffiecient in general, 
     but here it is only used to iterate over the list ONE BY ONE and pick one out *)
  | CMatch (dconAndNumArgs : list (dcon * nat))
@@ -141,12 +187,12 @@ Definition CPSOpBindings (c : L5Opid)
   match c with
   | CLambda    => [2] (* user lambda, also binds a continuation *)
   | CKLambda    => [1] (* continuation lambda  *)
-  | CFix nMut => repeat 1 nMut
+  | CFix nMut _ => repeat nMut nMut
   | CDCon _ nargs    => repeat 0 nargs
   | CHalt => [0]
   | CRet => [0,0]
   | CCall => [0,0,0]
-  | CProj _ => [0,0]
+(*  | CProj _ => [0,0] *)
   | CMatch numargsInBranches => 0::(List.map snd numargsInBranches)
   end.
 
@@ -204,12 +250,17 @@ Definition App_e (f a : NTerm) :=
 Definition Con_e (dc : dcon) (args : list NTerm) : NTerm :=
   oterm (NDCon dc (length args)) (List.map (bterm []) args).
 
+(*
 Definition Proj_e (arg : NTerm) (selector : nat)  : NTerm :=
   oterm (NProj selector) [bterm [] arg].
+*)
+
+Definition Fix_e' (lbt : list BTerm) (n:nat) : NTerm :=
+  oterm (NFix (length lbt) n) lbt.
 
 (** fix (\xf. (\x..,,)) *)
-Definition Fix_e (xf : NVar) (args : list NTerm) : NTerm :=
-  oterm (NFix (length args)) (List.map (bterm [xf]) args).
+Definition Fix_e (xf : list NVar) (args : list NTerm)  (n:nat) : NTerm :=
+  Fix_e' (List.map (bterm xf) args) n.
 
 Definition Match_e (discriminee : NTerm) (brs : list branch) : NTerm :=
   oterm (NMatch (List.map (fun b => (fst b, num_bvars (snd b))) brs))
@@ -262,9 +313,13 @@ Instance ExpSubstitute : Substitute NTerm NTerm :=
   { substitute := fun rep x t => subst t x rep}.
 
 
-Definition Fix_e' (lbt : list BTerm) : NTerm :=
-  oterm (NFix (length lbt)) lbt.
 
+Inductive is_value : NTerm -> Prop :=
+| var_is_value : forall i, is_value (vterm i)
+| lam_is_value : forall x e, is_value (Lam_e x e)
+| con_is_value : forall d es, (forall s, In s es -> is_value s) -> is_value (Con_e d es)
+(** Unlike in Nuprl, fix is a value.*)
+| fix_is_value : forall es n, is_value (Fix_e' es n).
 
 (** Big-step evaluation for [exp]. *)
 Inductive eval : NTerm -> NTerm -> Prop :=
@@ -275,7 +330,8 @@ Inductive eval : NTerm -> NTerm -> Prop :=
                  eval e2 v2 ->
                  eval (e1'{x := v2}) v -> 
                  eval (App_e e1 e2) v
-(**AA: do we need to go inside constructors for weak-head evaluation? *)
+(**AA: do we need to go inside constructors for weak-head evaluation? 
+What if we add coinductives? *)
 | eval_Con_e : forall d es vs, 
     length es = length vs
     -> (forall e v, (LIn (e,v) (combine es vs)) -> eval e v)
@@ -289,11 +345,33 @@ Inductive eval : NTerm -> NTerm -> Prop :=
                    find_branch d ((List.length vs)) bs = Some e' ->
                    eval (apply_bterm e' vs) v ->
                    eval (Match_e e bs) v
-| eval_Fix_e : forall es, eval (Fix_e' es) (Fix_e' es)
+| eval_Fix_e : forall es n, eval (Fix_e' es n) (Fix_e' es n)
+| eval_FixApp_e : forall e lbt n e2 v2 bt ev2,
+    let len := length lbt in
+    let pinds := (seq 0 len) in
+    let sub :=  (map (Fix_e' lbt) pinds) in
+    eval e (Fix_e' lbt n) ->
+    eval e2 v2 ->
+    select n lbt = Some bt ->
+    eval (App_e (apply_bterm bt sub) v2) ev2 ->
+    num_bvars bt = len ->
+    eval (App_e e e2) ev2.
+(* | eval_Ax_e s : eval (Ax_e s) (Ax_e s) 
+
 | eval_Proj_e : forall xf e es n xl bl,
                   eval e (Fix_e' es) ->
                   select n es = Some (bterm [xf] (Lam_e xl bl)) ->
                   eval (Proj_e e n) ((Lam_e xl bl){xf:=Fix_e' es}).
+
+*)
+
+Require Import Common.certiClasses.
+(* Enables the ⇓ notation.
+Local Instances are cleared at the end of a section.
+A more specific instance
+is redeclared in L4.instances using "Existing Instance" *)
+Local Instance L4aEval : BigStepOpSem NTerm := eval.
+
 
 (** will be used in [eval_reduces_fvars] and cps_cvt_corr *)
 Lemma subset_step_app: forall x e1' v2,
@@ -327,15 +405,42 @@ Qed.
 
 Local Opaque ssubst.
 
+(* will be used in eval_reduces_fvars and cps_cvt_corr *)
+Lemma subset_fvars_fix : forall bt lbt,
+LIn bt lbt ->
+Datatypes.length (get_vars bt) = Datatypes.length lbt ->
+let len := Datatypes.length lbt in
+let pinds := seq 0 len in
+let sub := map (Fix_e' lbt) pinds in
+subset (free_vars (apply_bterm bt sub)) (flat_map free_vars_bterm lbt).
+Proof using.
+  intros ? ? Hin Hl. simpl.  
+  unfold apply_bterm.
+  rewrite eqsetv_free_vars_disjoint.
+  intros v Hc.
+  rewrite in_app_iff in Hc.
+  rewrite dom_sub_combine in Hc;
+    [ | rewrite map_length, seq_length; assumption].
+  dorn Hc; [rewrite  in_flat_map; simpl; exists bt; destruct bt; eauto | ].
+  apply in_sub_free_vars in Hc.
+  exrepnd.
+  apply in_sub_keep_first in Hc0.
+  repnd.
+  apply sub_find_some in Hc2.
+  apply in_combine in Hc2.
+  apply proj2 in Hc2.
+  apply in_map_iff in Hc2.
+  exrepnd. subst. clear Hc2.
+  assumption.
+Qed.
+
 Lemma eval_reduces_fvars :
-  forall e v, eval e v ->  subset (free_vars v) (free_vars e).
+  forall (e v : NTerm) , e ⇓ v -> subset (free_vars v) (free_vars e).
 Proof using.
   intros ? ? He. unfold closed. induction He; try auto;
   simpl in *;autorewrite with core list in *.
   (**Apply case*)
-  -
-    unfold subset.
-    pose proof (subset_step_app x e1' v2) as H.
+  - pose proof (subset_step_app x e1' v2) as H.
     pose proof (subset_trans _ _ _ _ IHHe3 H).
     clear H IHHe3. eapply subset_trans; eauto.
     simpl. autorewrite with list core.
@@ -384,22 +489,18 @@ Proof using.
       apply sub_find_some in Hf0. apply in_combine_r in Hf0.
       assumption.
 
-- intros ? Hf. unfold subst.
-  apply_clear IHHe. unfold subst in Hf.
-  rewrite eqsetv_free_vars_disjoint in Hf.
-   simpl in Hf.
-  rewrite in_app_iff in *.
-  dorn Hf. 
-  + unfold compose. repnd.
-    apply select_in in H. apply in_flat_map. eexists; split; eauto.
-  + rewrite memvar_dmemvar in Hf. 
-    if_splitH Hf; simpl in Hf; autorewrite with list in *;[|firstorder].
-    assumption.
+(* fix application *)
+- eapply subset_trans; eauto.
+  apply subsetvAppLR; auto.
+  eapply subset_trans; [| apply IHHe1].
+  clear He3 IHHe3.
+  apply select_in in H.
+  apply subset_fvars_fix; auto.
 Qed.
 
 (** Evaluation preserves closedness.*)
 Corollary eval_preserves_closed :
-  forall e v, eval e v ->  closed e -> closed v.
+  forall (e v : NTerm),  e ⇓ v ->  closed e -> closed v.
 Proof using.
   intros ? ?  He. unfold closed. intro Hc.
   apply eval_reduces_fvars  in He.
@@ -408,20 +509,15 @@ Proof using.
 Qed.
 
 (** Characterize values *)
-Inductive is_value : NTerm -> Prop :=
-| var_is_value : forall i, is_value (vterm i)
-| lam_is_value : forall x e, is_value (Lam_e x e)
-| con_is_value : forall d es, (forall s, In s es -> is_value s) -> is_value (Con_e d es)
-(** Unlike in Nuprl, fix is a value.*)
-| fix_is_value : forall es, is_value (Fix_e' es).
+
 
 (** Show that evaluation always yields a value. *)
 Lemma eval_yields_value' :
   (forall e v, eval e v -> is_value v).
 Proof using.
   intros ? ? He ; induction He ; simpl ; intros;
-  auto ; try constructor ; auto;[|].
-  - change vs  with (snd (es, vs)).
+  auto ; try constructor ; auto.
+  change vs  with (snd (es, vs)).
     rename H into Hl.
     apply combine_split in Hl.
     rewrite <- Hl.
@@ -430,16 +526,26 @@ Proof using.
     apply in_map_iff in Hin.
     exrepnd. simpl in *. subst.
     eauto.
-  - unfold subst.
-    Local Transparent ssubst. unfold Lam_e. unfold ssubst. simpl.
-    cases_ifd Hd; simpl;[constructor|].
-    unfold freshReplacements. simpl in *.
-    addFreshVarsSpec2 lvn Hfr.
-    repnd. simpl in *. dlist_len_name lvn a. simpl. constructor. 
 Qed.
 
 Ltac ntwfauto := 
 simpl substitute in *;alphaeq.ntwfauto.
+
+
+
+Lemma fVarsFix' : forall lbt,
+eq_set
+  (flat_map all_vars (map (Fix_e' lbt) (seq 0 (Datatypes.length lbt))))
+  (flat_map all_vars_bt lbt).
+Proof using.
+  intros. rewrite flat_map_map.
+  unfold compose.
+  unfold Fix_e'.
+  rewrite eqset_flat_maps with (g:= fun x => (flat_map all_vars_bt lbt));
+    [| intros ? ?; rewrite all_vars_ot at 1; refl].
+  destruct lbt;[refl | ].
+  apply eqset_repeat. simpl. discriminate.
+Qed.
 
 Lemma eval_preseves_wf :
   forall e v, eval e v ->  nt_wf e -> nt_wf v.
@@ -466,11 +572,14 @@ Proof using.
   + apply find_branch_some in H. repnd.
     repnd. rewrite <- (bt_wf_iff l).
     apply Hntwf. auto.
-- ntwfauto. 
-  subst.
-  apply select_in in H.
-  apply Hntwf in H.
+- unfold len, sub, pinds in *.
   ntwfauto.
+  apply IHHe3.
+  ntwfauto.
+  + apply in_combine in Hsub. repnd. apply in_map_iff in Hsub.
+    exrepnd. subst. ntwfauto.
+  + apply select_in in H. destruct bt. ntwfauto.
+  + rewrite or_false_r in HntwfIn. subst. ntwfauto.  
 Qed.
 
 
@@ -535,21 +644,22 @@ Proof using.
   rewrite allvars_bterm.
   apply in_app_iff. tauto.
 
-- remember (Lam_e xl bl) as r. clear Heqr.
-  unfold Fix_e', Proj_e in *.
-  apply ssubst_allvars_varclass_nb.
-  apply select_in in H.
-  rwsimplAll.
-  split;[| tauto].
+- unfold Fix_e, Fix_e', App_e,  sub, pinds, len in *.
+  apply_clear IHHe3.
+  rwsimplC.
+  rwsimpl Hn.
+  rwsimpl IHHe1.
   repnd.
-  eapply varsOfClassSubset;[| apply IHHe; auto].
-  intros ? Hin.
-  apply in_flat_map. eexists.
-  split;[apply H|].
-  unfold compose.
-  simpl.
-  rewrite allvars_bterm.
-  apply in_app_iff. tauto.
+  dands; eauto with SquiggleEq;[].
+  repnd.
+  apply ssubst_allvars_varclass_nb.
+  rewrite dom_range_combine;[| destruct bt; autorewrite with list; auto ].
+  apply select_in in H.
+  rwsimpl IHHe1.
+  apply varsOfClassApp.
+  dands;[destruct bt; simpl in *;eauto with subset | ].
+  rewrite fVarsFix'.
+  auto 2.
 Qed.
 
 
@@ -575,15 +685,20 @@ Definition Call_c (f k a : CTerm) :=
 Definition Con_c (dc : dcon) (args : list CTerm) : CTerm :=
   coterm (CDCon dc (length args)) (List.map (bterm []) args).
 
+(*
 Definition Proj_c (arg: CTerm) (selector : nat) (cont: CTerm)  : CTerm :=
   coterm (CProj selector) [bterm [] arg, bterm [] cont].
+*)
 
-(** do we need a continuation variable as well? *)
-Definition Fix_c (xf : NVar) (args : list CTerm) : CTerm :=
-  coterm (CFix (length args)) (List.map (bterm [xf]) args).
+Definition Fix_c' (lbt : list CBTerm) (n:nat) : CTerm :=
+  coterm (CFix (length lbt) n) lbt.
 
-Definition Fix_c' (lbt : list CBTerm) : CTerm :=
-  coterm (CFix (length lbt)) lbt.
+(** do we need a continuation variable as well? 
+A continuation variable is only needed for elim forms. a Fix is eliminated using an App.
+*)
+Definition Fix_c (xf : list NVar) (args : list CTerm) (n:nat) : CTerm :=
+  Fix_c' (List.map (bterm xf) args) n.
+
 
 Definition Match_c (discriminee : CTerm) (brs : list branch) : CTerm :=
   coterm (CMatch (List.map (fun b => (fst b, num_bvars (snd b))) brs))
@@ -593,7 +708,7 @@ Definition Match_c (discriminee : CTerm) (brs : list branch) : CTerm :=
 Instance CExpSubstitute : Substitute CTerm CTerm :=
   { substitute := fun rep x t => subst t x rep}.
 
-
+Print eval.
 (** OPTIMISED Big-step evaluation for CPS expressions.
     Notice that only computations
     are evaluated -- values are inert so to speak. *)
@@ -606,7 +721,8 @@ Inductive eval_c : CTerm -> CTerm -> Prop :=
 | eval_Call_c : forall xk x c v1 v2 v',
                   eval_c (ssubst c [(x,v2);(xk,v1)]) v' -> 
                   eval_c (Call_c ((Lam_c x xk c)) v1 v2) v'
-| eval_Match_c : forall d vs bs c v',
+
+| eval_Match_c :  forall d vs bs c v',
                    find_branch d (List.length vs) bs = Some c ->
                    eval_c (apply_bterm c vs) v' -> 
                    eval_c (Match_c (Con_c d vs) bs) v'
@@ -617,11 +733,15 @@ Inductive eval_c : CTerm -> CTerm -> Prop :=
                   eval_c (Ret_c k (fn{xf:=Fix_c' lbt})) v' ->  
                   eval_c (Proj_c (Fix_c' lbt) i k) v'. *)
 
-| eval_Proj_c : forall lbt i k v' xf fn, 
-(* fn is a value, which will have a val_outer (defined below) in the intended usecase*)
-                  select i lbt = Some (bterm [xf] fn) -> 
-                  eval_c (Ret_c (fn{xf:=Fix_c' lbt}) k) v' ->
-                  eval_c (Proj_c (Fix_c' lbt) i k) v'.
+(* fn is a lambda *)
+| eval_FixApp_c : forall lbt i k arg v bt, 
+    let len := Datatypes.length lbt in
+    let pinds := seq 0 len in
+    let sub := map (Fix_c' lbt) pinds in
+    select i lbt = Some bt -> 
+    eval_c (Call_c (apply_bterm bt sub) k arg) v ->
+    eval_c (Call_c (Fix_c' lbt i) k arg) v.
+
 Hint Constructors eval_c.
 
 (** Useful for rewriting. *)
@@ -687,10 +807,10 @@ Fixpoint is_valueb (e:NTerm) : bool :=
       match c with
           (* expensive test. need memoization *)
         | NLambda => true
-        | NFix _ => true
+        | NFix _ _ => true
         | NDCon _ _ => ball (List.map (is_valueb ∘ get_nt) lb)
         | NApply => false
-        | NProj _ => false
+(*        | NProj _ => false *)
         | NLet => false
         | NMatch _ => false
       end
@@ -767,11 +887,11 @@ Section CPS_CVT.
              (Lam_c x kv (Ret_c (cps_cvt b) (vterm kv))).
 
   (** the KLam_c was manually added. unlike now, Fix_c previously implicitly bound a var*)
-  Definition cps_cvt_fn_list'  (es: list BTerm) : list CBTerm :=
+  Definition cps_cvt_fn_list' f (es: list BTerm) : list CBTerm :=
     map (fun b => 
             let e := get_nt b in
             let vars := get_vars b in
-                    bterm vars (cps_cvt e)) es.
+                    bterm vars (f e)) es.
 
   Fixpoint cps_cvt_val' (e:NTerm) : CTerm :=
     match e with
@@ -783,9 +903,9 @@ Section CPS_CVT.
                       bterm []
                             (cps_cvt_val' (get_nt b))) in
             coterm (CDCon d l) (List.map fb lb)
-      | terms.oterm (NFix nargs) lb =>
-          coterm (CFix nargs)
-             (cps_cvt_fn_list' lb)
+      | terms.oterm (NFix nargs i) lb =>
+          coterm (CFix nargs i)
+             (cps_cvt_fn_list' cps_cvt_val' lb)
       | _ => coterm CLambda (map ((bterm []) ∘ vterm)  (free_vars e))
           (* ill-formed term, which will not arise from the prev. phase.
             This choice, which is also ill-formed,
@@ -848,12 +968,12 @@ Fixpoint cps_cvt (e:NTerm) {struct e}: CTerm :=
       let cpsLam := (val_outer (cps_cvt_lambda cps_cvt x e2)) in
         cps_cvt_apply cps_cvt cpsLam e1
 
-    | terms.oterm (NProj i) [bterm [] e] =>
+(*    | terms.oterm (NProj i) [bterm [] e] =>
       let kvars := contVars  2 in 
       let k := nth 0 kvars nvarx in  
       let ke := nth 1 kvars nvarx in  
         KLam_c k (Ret_c (cps_cvt e) 
-                        (KLam_c ke (Proj_c (vterm ke) i (vterm k))))
+                        (KLam_c ke (Proj_c (vterm ke) i (vterm k)))) *)
     | _ => coterm CLambda (map ((bterm []) ∘ vterm)  (free_vars e))
           (* ill-formed term, which will not arise from the prev. phase.
             This choice, which is also ill-formed,
@@ -1095,6 +1215,7 @@ Definition cps_cvt_apply_step : Prop := forall e1 e2 :NTerm,
 
 End CPS_CVT_INDUCTION.
 
+(* TODO : pick an appropriate name *)
 Local Lemma cps_cvt_val_aux_fvars_aux : forall o lbt,
   (forall es, 
     (size es) < size (oterm o lbt)
@@ -1104,6 +1225,37 @@ Local Lemma cps_cvt_val_aux_fvars_aux : forall o lbt,
 -> nt_wf (oterm o lbt)
 -> varsOfClass (all_vars (oterm o lbt)) USERVAR
 -> eq_set (flat_map free_vars_bterm (cps_cvt_fn_list' cps_cvt lbt))
+          (flat_map free_vars_bterm lbt).
+Proof using.
+  intros ? ? Hyp  Hwf Hvc.
+  unfold cps_cvt_fn_list'. rewrite flat_map_map.
+  apply eqset_flat_maps.
+  intros bt Hin.
+  destruct bt as [lvb nt]. unfold compose.
+  simpl.
+  autorewrite with list SquiggleEq.
+  autorewrite with list in *.
+  varsOfClassSimpl.
+  rewrite Hyp; [
+    | eapply size_subterm3; eauto
+    | ntwfauto
+    | tauto
+      ].
+  apply proj2, userVarsContVar in Hin.
+  refl.
+Qed.
+
+(* TODO : pick an appropriate name *)
+
+Local Lemma cps_cvt_val_aux_fvars_aux2 : forall o lbt,
+  (forall es, 
+    (size es) < size (oterm o lbt)
+    -> nt_wf es 
+    -> varsOfClass (all_vars es) USERVAR
+    -> eq_set (free_vars (cps_cvt_val  es)) (free_vars es))
+-> nt_wf (oterm o lbt)
+-> varsOfClass (all_vars (oterm o lbt)) USERVAR
+-> eq_set (flat_map free_vars_bterm (cps_cvt_fn_list' cps_cvt_val lbt))
           (flat_map free_vars_bterm lbt).
 Proof using.
   intros ? ? Hyp  Hwf Hvc.
@@ -1142,10 +1294,10 @@ Lemma cps_cvt_val_aux_fvars :
   cps_cvt_val_step cps_preserves_fvars.
 Proof using.
   simpl. unfold cps_preserves_fvars. intros ? Hyp.
-  nterm_ind e as [v | o lbt Hind] Case;[eauto|].
+  induction e as [v | o lbt Hind] using NTerm_better_ind3;[eauto|].
   intros Hwf Hs. simpl in Hs.
   destruct o; try illFormedCase;
-    [clear Hind| clear Hind|]; inverts Hwf as Hbt Hnb;
+    [clear Hind| |]; inverts Hwf as Hbt Hnb;
     simpl in Hnb.
 (* lambda case *)
 - simpl.
@@ -1164,7 +1316,9 @@ Proof using.
   auto.
 (* Fix_e case *)
 - simpl.
-  eapply cps_cvt_val_aux_fvars_aux; eauto.
+  eapply cps_cvt_val_aux_fvars_aux2; eauto;[| ntwfauto].
+  intros. eapply Hind; eauto.
+  intros. eapply Hyp; eauto. omega.
   
 (* Con_e case *)
 - simpl.
@@ -1176,8 +1330,8 @@ Proof using.
   unfold num_bvars in Hnb. simpl in Hnb.
   dlist_len_name l vv.
   apply properEqsetvRemove; eauto.
-  rewrite Hind; eauto; [|ntwfauto; fail|].
-  + intros.  apply Hyp; eauto. eapply lt_trans; eauto.
+  rewrite Hind; eauto;[eauto using size_subterm3 | | ntwfauto |].
+  + intros.  apply Hyp; eauto.  eapply lt_trans; eauto.
     eapply size_subterm3; eauto.
   + varsOfClassSimpl. tauto.
 Qed.
@@ -1344,17 +1498,6 @@ Local Transparent cps_cvt_val' is_valueb.
     unfold cps_preserves_fvars.
     intros; apply Hind; auto;[]. simpl in *. omega.
 
-(** Proj_e *)
-  + dnumvbars Hnb bt. unfold num_bvars. simpl.
-    addContVarsSpec 2 Hs kv. repnd.
-    simpl in *. dlist_len_name lkv kv; simpl in *.
-    repeat progress (autorewrite with list SquiggleEq SquiggleEq2 in *; simpl in * ).
-    rewrite remove_nvars_nops;[|noRepDis].
-    autorewrite with list SquiggleEq.
-    autorewrite with  SquiggleEq in Hs.
-    rewrite Hind;[| omega | ntwfauto | tauto].
-    autorewrite with list SquiggleEq.
-    rewrite remove_nvars_nop;[auto| inauto; eauto].
 
 (** Let_e *)
   + dnumvbars Hnb b.
@@ -1478,19 +1621,19 @@ Qed.
 Lemma isvalueb_ssubst_aux : forall t sub,
 sub_range_sat sub is_value 
 -> (is_valueb (ssubst_aux t sub)) = is_valueb t.
-Proof.
+Proof using.
   intro t. induction t as [v | o lbt Hind] using NTerm_better_ind; intros ? Hsr.
 - simpl. dsub_find sf;[| refl]; symmetry in Heqsf.
   apply is_valueb_corr.  eapply Hsr. apply sub_find_some. eauto.
 - simpl. destruct o; try refl.
-  rewrite map_map.
-  f_equal.
-  apply eq_maps.
-  intros bt Hin.
-  destruct bt as [lv nt].
-  unfold compose.
-  simpl.
-  eapply Hind; eauto.
+   rewrite map_map.
+    f_equal.
+    apply eq_maps.
+    intros bt Hin.
+    destruct bt as [lv nt].
+    unfold compose.
+    simpl.
+    eapply Hind; eauto.
 Qed.
 
 
@@ -1514,7 +1657,7 @@ Hint Constructors is_value : CerticoqCPS.
 Lemma isvalue_ssubst_aux : forall t sub,
 sub_range_sat sub is_value 
 -> (is_value (ssubst_aux t sub)) <-> is_value t.
-Proof.
+Proof using.
   intro t. induction t as [v | o lbt Hind] using NTerm_better_ind; intros ? Hsr.
 - simpl. dsub_find sf;[| refl]; symmetry in Heqsf.
   apply sub_find_some in Heqsf. apply Hsr in Heqsf.
@@ -1552,9 +1695,35 @@ Qed.
 *)
 Hint Rewrite isvalueb_ssubst_aux : CerticoqCPS.
 
+Definition is_lambdab (n: NTerm) :=
+decide (getOpid n = Some NLambda).
+
+
+Fixpoint fixwf (e:NTerm) : bool :=
+match e with
+| terms.vterm _ => true (* closedness is a the concern of this predicate *) 
+| terms.oterm o lb => 
+    (match o with
+    | NFix _ _ => ball (map (is_lambdab ∘ get_nt) lb) 
+    | _ => true
+    end) && ball (map (fixwf ∘ get_nt) lb)
+end.
+
+
+Lemma is_lambdab_is_valueb : forall t,
+  is_lambdab t = true -> is_valueb t = true.
+Proof using.
+  intros ? H. destruct t as [? | o ? ]; auto.
+  destruct o; inverts H.
+  refl.
+Qed.
+
+
+
 Definition cps_ssubst_commutes (e : NTerm) (cps_cvt' : NTerm -> CTerm) := 
   forall (sub : Substitution),
 nt_wf e
+-> (fixwf e = true)
 -> sub_range_sat sub is_value (* can we get rid of this ?*)
 -> sub_range_sat sub nt_wf
 -> sub_range_sat sub closed
@@ -1565,13 +1734,13 @@ nt_wf e
 Lemma val_outer_ssubst_aux : forall t sub,
 disjoint [contVar] (dom_sub sub)
 ->ssubst_aux (val_outer t) sub = val_outer (ssubst_aux t sub).
-Proof.
+Proof using.
   intros ? ? Hdis. unfold val_outer.
   simpl. unfold KLam_c, Ret_c.
   autorewrite with SquiggleEq.
   rewrite sub_filter_disjoint1; [|disjoint_reasoningv2].
   repeat f_equal.
- rewrite sub_find_none_if;
+  rewrite sub_find_none_if;
      [refl|disjoint_reasoningv2].
 Qed.
 
@@ -1580,7 +1749,7 @@ Hint Resolve sub_filter_subset flat_map_monotone varsOfClassSubset map_monotone 
 *)
 
 Lemma contVars1 : contVars 1 = [contVar].
-Proof.
+Proof using.
   unfold contVar, contVars.
   addFreshVarsSpec2 lvn Hfr.
   simpl in *. repnd.
@@ -1593,10 +1762,10 @@ Lemma cps_cvt_val_ssubst_commutes_aux :
 Proof using.
   simpl. unfold cps_ssubst_commutes. intros ? Hyp.
   nterm_ind e as [v | o lbt Hind] Case;
-  intros Hev ?  Hwf Hisv Hwfs Hcs  Hs;
+  intros Hev ?  Hwf Hfwf Hisv Hwfs Hcs  Hs;
   applydup userVarsContVar in Hs as Hdisvc; simpl in Hdisvc;
   [ | destruct o; try (complete (inverts Hev)) ; inverts Hwf as Hbt Hnb; simpl in Hnb];
-    [| clear Hind | clear Hind| ].
+    [| clear Hind  | | ].
 - simpl. symmetry.
   dsub_find sf; symmetry in Heqsf; [|erewrite sub_find_none_map; eauto; fail].
   erewrite sub_find_some_map; eauto.
@@ -1614,9 +1783,12 @@ Proof using.
   rewrite (sub_filter_disjoint1 sub); [|disjoint_reasoningv2].
   rwsimpl Hs.
   simpl in Hbt. dLin_hyp.
+  simpl in Hfwf. apply andb_true_iff, proj1 in Hfwf.
+  unfold compose in Hfwf. simpl in Hfwf.
   apply Hyp; auto; simpl; try omega; try ntwfauto.
   repnd.
   rwsimplC. dands; unfold range, dom_sub, dom_lmap; eauto with subset.
+(* Fix case *)
 - simpl. f_equal. setoid_rewrite map_map.
   apply eq_maps.
   intros bt Hin.
@@ -1626,9 +1798,20 @@ Proof using.
   autorewrite with SquiggleEq.
   rewrite sub_filter_map_range_comm.
   rwsimpl Hs.
-  apply Hyp; auto; simpl;[eapply size_subterm4; eauto | ntwfauto|].
+  simpl in Hfwf.  apply andb_true_iff in Hfwf.
+  repeat rewrite ball_map_true in Hfwf.
   repnd.
-  rwsimplC. dands; unfold range, dom_sub, dom_lmap; eauto with subset.
+  specialize (Hfwf0 _ Hin).
+  specialize (Hfwf _ Hin).
+  unfold compose in *. simpl in *.
+  apply is_lambdab_is_valueb in Hfwf0.
+  apply Hind with (lv:=lv); auto; simpl;
+    [ |  ntwfauto |  ].
+  + intros.  apply Hyp; eauto. eapply lt_trans; eauto.
+    eapply size_subterm4; eauto.
+  + repnd. repeat rewrite varsOfClassApp.
+    unfold dom_sub, dom_lmap, range. (* unfolding makes the lemmas in hintdb applicable *)
+    dands; eauto with subset.
 - simpl. f_equal. setoid_rewrite map_map.
   apply eq_maps.
   intros bt Hin.
@@ -1642,6 +1825,10 @@ Proof using.
   rewrite ball_map_true in Hev. unfold compose in Hev.
   applydup_clear Hev in Hin.
   simpl in *.
+  simpl in Hfwf.
+  repeat rewrite ball_map_true in Hfwf.
+  specialize (Hfwf _ Hin).
+
   apply Hind with (lv:=[]); auto;[| ntwfauto|].
   + intros.  apply Hyp; eauto. eapply lt_trans; eauto.
     eapply size_subterm4; eauto.
@@ -1654,7 +1841,7 @@ Qed.
 Lemma cps_cvt_apply_ssubst_commutes_aux : 
   cps_cvt_apply_step cps_ssubst_commutes.
 Proof using.
-  intros ? ? Hind ? Hwf H1s H2s H3s Hs. 
+  intros ? ? Hind ? Hwf Hfwf H1s H2s H3s Hs. 
   simpl. unfold cps_cvt_apply. simpl.
   addContVarsSpec 3 Hs kv. repnd. clear Heqlvcvf.
   simpl in *.
@@ -1670,6 +1857,8 @@ Proof using.
   rwsimpl  Hs.
   pose proof (size_pos e1).
   pose proof (size_pos e2).
+  unfold compose in Hfwf. simpl in Hfwf.
+  repeat rewrite andb_true_iff in Hfwf. repnd.
   do 4 f_equal;[| do 5 f_equal];
     (apply Hind; auto; [try omega| ntwfauto | rwsimplC; try tauto]).
 Qed.
@@ -1684,7 +1873,7 @@ sub_range_sat sub is_value (* can we get rid of this ?*)
      (size es <  S (addl (map size_bterm lbt)))
       -> cps_ssubst_commutes es cps_cvt)
   -> length lbt = length lkv
-  -> (forall b, LIn b lbt -> (bt_wf b /\ get_vars b = []))
+  -> (forall b, LIn b lbt -> (bt_wf b /\ get_vars b = [] /\ fixwf (get_nt b)=true))
     -> varsOfClass (flat_map all_vars_bt lbt) USERVAR 
     -> disjoint (lkv++free_vars c) (dom_sub sub)
    -> let sf := (map_sub_range (cps_cvt_val' cps_cvt) sub) in
@@ -1704,7 +1893,7 @@ Proof using.
     simpl in * ).
   unfold Ret_c, KLam_c.
   do 3 f_equal;[|do 4 f_equal].
-+ apply Hyp; auto;[ omega | ntwfauto | rwsimplC; tauto].
++ apply Hyp; auto;[ omega | ntwfauto  | rwsimplC; tauto].
 + rewrite sub_filter_map_range_comm.
   rewrite (sub_filter_disjoint1 sub); [|disjoint_reasoningv2].
   rewrite IHlbt; simpl;
@@ -1713,13 +1902,14 @@ Proof using.
 Qed.
 
 
+(* TODO : rename [cps_cvt/eval_c] *)
 Lemma eval_c_ssubst_aux_commute : forall (e : NTerm),
-  cps_ssubst_commutes e cps_cvt.
+cps_ssubst_commutes e cps_cvt.
 Proof using.
 Local Opaque is_valueb cps_cvt_val'.
   intros ?. unfold closed.
   induction e as [xx | o lbt Hind] using NTerm_better_ind3;
-  intros ?  Hwf Hisv Hwfs Hcs  Hs;
+  intros ?  Hwf Hfwf Hisv Hwfs Hcs  Hs;
   applydup userVarsContVar in Hs as Hdisvc; simpl in Hdisvc;
   [ | simpl; 
       setoid_rewrite (isvalueb_ssubst_aux (oterm o lbt) sub);
@@ -1733,13 +1923,14 @@ Local Transparent is_valueb.
     [| autorewrite with SquiggleEq; disjoint_reasoningv2].
   f_equal. apply cps_cvt_val_ssubst_commutes_aux; auto. simpl.
   intros es ?. pose proof (size_pos es). omega.
-(* value oterm *)
+(*legal value oterm *)
 - 
 Local Opaque is_valueb.
 Local Transparent ssubst_aux.
   rewrite val_outer_ssubst_aux;
     [| autorewrite with SquiggleEq; disjoint_reasoningv2].
   f_equal. apply cps_cvt_val_ssubst_commutes_aux; auto.
+
 (* constructor*)
 - simpl. unfold KLam_c. autorewrite with list SquiggleEq. 
   do 3 f_equal. clear H0. clear Hdisvc.
@@ -1753,10 +1944,10 @@ Local Transparent ssubst_aux.
   rewrite (sub_filter_disjoint1 sub); [|disjoint_reasoningv2].
   unfold num_bvars in Hnb.
   setoid_rewrite length_zero_iff_nil in Hnb.
+  rewrite ball_map_true in Hfwf. unfold compose in Hfwf.
   rewrite cps_cvt_constr_subst_aux; auto;
     [ rwsimplC; try tauto
-      | simpl; rwsimplC; disjoint_reasoningv2].
-
+      |  simpl; rwsimplC; disjoint_reasoningv2].
 Local Transparent is_valueb.
 
 (* App_e *)
@@ -1766,22 +1957,6 @@ Local Transparent is_valueb.
   rewrite cps_cvt_apply_ssubst_commutes_aux; auto; [|ntwfauto].
   simpl in *.
   intros. apply Hind. omega.
-(* Proj_e *)
-- dnumvbars Hnb bt. unfold num_bvars. simpl.
-  addContVarsSpec 2 Hs kv. repnd. clear Heqlvcvf.
-  simpl.
-  rwsimplC.
-  unfold KLam_c, Ret_c.
-  do 4 f_equal.
-  do 2 (rewrite sub_filter_map_range_comm;
-        rewrite (sub_filter_disjoint1 sub); [|disjoint_reasoningv2]).
-  do 2 (rewrite (sub_find_none_if); 
-          [| rwsimplC ; apply disjoint_singleton_l; disjoint_reasoningv2]).
-  do 2 f_equal.
-  simpl in *.
-  dLin_hyp.
-  rwsimpl Hs.
-  apply Hind; auto;[omega| ntwfauto | rwsimplC; tauto].
 
 (* Let_e *)
 - 
@@ -1790,15 +1965,19 @@ Local Transparent is_valueb.
     with (cps_cvt ((Let_e btlv0 btnt btnt0))).
   rewrite cps_cvt_let_as_app_lam.
   rwsimpl Hs.
+  simpl in Hfwf. repeat rewrite andb_true_iff in Hfwf.
+  unfold compose in Hfwf. simpl in Hfwf. dands.
   rewrite cps_cvt_apply_ssubst_commutes_aux; unfold Lam_e, App_e in *;
-    simpl in *;auto;
+    simpl in *;auto; unfold compose; simpl; unfold compose; simpl;
     [ | intros; apply Hind; auto; omega 
       | ntwfauto 
+      | repnd; rwHyps; refl
       | rwsimplC; dands; try tauto].
   autorewrite with SquiggleEq.
   refl.
-- 
-  dnumvbars Hnb bt. unfold num_bvars. simpl.
+
+(* match *)
+- dnumvbars Hnb bt. unfold num_bvars. simpl.
   addContVarsSpec 2 Hs kv. repnd. clear Heqlvcvf.
   simpl. unfold KLam_c, Ret_c.
   do 4 f_equal.
@@ -1810,6 +1989,8 @@ Local Transparent is_valueb.
   simpl in *.
   dLin_hyp.
   rwsimpl Hs.
+  unfold compose in Hfwf.
+  repeat rewrite andb_true_iff in Hfwf. simpl in Hfwf. repnd.
   do 2 f_equal;[| do 6 f_equal];
     [ apply Hind; auto;[omega| ntwfauto | rwsimplC; tauto] |].
   setoid_rewrite map_map.
@@ -1829,6 +2010,8 @@ Local Transparent is_valueb.
   repnd.
   pose proof Hin as Hins.
   apply size_subterm4 in Hins.
+  rewrite ball_map_true in Hfwf.
+  specialize (Hfwf _ Hin).
   apply Hind; auto;[omega| ntwfauto | rwsimplC; dands; 
     unfold range, dom_sub, dom_lmap; eauto with subset].
 Qed.
@@ -1874,6 +2057,7 @@ Abort.
 
 Lemma eval_c_ssubst_commute : forall (e : NTerm) (sub : Substitution) ,
 nt_wf e
+-> fixwf e = true
 -> sub_range_sat sub is_value (* can we get rid of this ?*)
 -> sub_range_sat sub nt_wf
 -> sub_range_sat sub closed
@@ -1881,7 +2065,7 @@ nt_wf e
 ->  let sub_c := (map_sub_range (cps_cvt_val' cps_cvt)) sub in
       (ssubst (cps_cvt e) sub_c)= (cps_cvt (ssubst e sub)).
 Proof using.
-  intros.
+  intros ? ? Hfwf. intros.
   change_to_ssubst_aux8;[apply eval_c_ssubst_aux_commute; assumption|].
   subst sub_c.
   rewrite disjoint_flat_map_r.
@@ -1945,7 +2129,7 @@ Lemma val_outer_ssubst : forall t sub,
 (flat_map free_vars (range sub)) = []
 -> disjoint [contVar] (dom_sub sub)
 -> ssubst (val_outer t) sub = val_outer (ssubst t sub).
-Proof.
+Proof using.
   intros ? ? H1dis H2dis.
   change_to_ssubst_aux8; try rewrite H1dis; auto.
   apply val_outer_ssubst_aux. auto.
@@ -1959,118 +2143,96 @@ Ltac prepareForEvalRet Hc Hs :=
         (intros ? ? ?; in_reasoning; cpx)]
   end.
 
-Lemma cps_cvt_corr_app_let_common_part:
-forall 
-(x kv kv0 kv1 : NVar)
-(e2 e1' v2 v : NTerm)
-(k v' : CTerm)
-(Hvc : varsOfClass (all_vars e2 ++ [x] ++ all_vars e1' ++ all_vars v2) USERVAR)
-(He1 : eval e2 v2)
-(He2 : eval (ssubst e1' [(x, v2)]) v)
-(IHHe2 : forall k : CTerm,
-        free_vars k = [] -> forall v' : CTerm, eval_c (Ret_c (cps_cvt e2) k) v' <-> eval_c (Ret_c (cps_cvt v2) k) v')
-(Hcle : isprogram e2 /\ isprogram_bt (bterm [x] e1') /\ closed k /\ closed v2)
-(Hvcnr : no_repeats [kv, kv0, kv1])
-(Hcvdis : disjoint [contVar, kv, kv0, kv1] (all_vars e2 ++ x :: all_vars e1')) 
-(Hcsss : (closed (KLam_c kv0 (Ret_c (cps_cvt e2) (KLam_c kv1 (Call_c (vterm kv0) k (vterm kv1))))))),
-eval_c
-  (Ret_c (val_outer (cps_cvt_lambda cps_cvt x e1'))
-     (KLam_c kv0 (Ret_c (cps_cvt e2) (KLam_c kv1 (Call_c (vterm kv0) k (vterm kv1)))))) v' <->
-eval_c (Ret_c (cps_cvt (ssubst e1' [(x, v2)])) k) v'.
-Proof using.
-  intros. unfold isprogram, isprogram_bt, closed, closed_bt in *. repnd.
-  rwsimpl Hvc. simpl in *.
-  unfold  val_outer, cps_cvt_lambda.
-  rewrite eval_ret. simpl.
-  unfold subst.
-  rewrite ssubstRet_c by assumption.
-  rewrite ssubst_vterm. simpl ssubst_aux.
-  progress autorewrite with SquiggleEq.
-  match goal with
-  [|- context [Ret_c _ (ssubst ?k _)]] => assert (closed k) as Hclk;
-    [|  assert (sub_range_sat [(kv0 , k)] closed) as Hcs by
-        (intros ? ? ?; in_reasoning; cpx)]
-  end.
-    unfold closed. simpl. autorewrite with list core SquiggleEq.
-    symmetry.
-    rewrite cps_cvt_aux_fvars;
-      [| apply' eval_preseves_wf He1; ntwfauto; fail
-       | try tauto].
-    rewrite remove_nvars_app_r.
-    rewrite cons_as_app.
-    repeat rewrite <- remove_nvars_app_l.
-    autorewrite with SquiggleEq.
-    rewrite remove_nvars_comm. rwHyps. refl.
+Let  evalt := fun e v =>
+(forall k, closed k ->
+    forall v',
+      eval_c (Ret_c (cps_cvt e) k) v' <->
+        eval_c (Ret_c (cps_cvt v) k) v') /\ eval e v.
 
-  rewrite substLam_cTrivial2 by assumption.
-  rewrite eval_ret. simpl.
-  unfold subst.
+Hint Unfold isprogram : eval.
+Hint Resolve eval_yields_value' eval_preseves_varclass 
+  eval_preseves_wf eval_preserves_closed conj
+  cps_cvt_val_closed cps_cvt_closed : eval.
+
+Lemma cps_cvt_apply_eval : forall e e2 ev2 ev k v
+(Hp : isprogram e /\ isprogram e2)
+(Hclk : closed k)
+(Hvc : varsOfClass (all_vars e ++ all_vars e2) USERVAR)
+(H1e : evalt e ev)
+(H2e : evalt e2 ev2),
+(eval_c (Ret_c (cps_cvt_apply cps_cvt (cps_cvt e) e2) k) v
+<->
+eval_c (Call_c (cps_cvt_val ev) k (cps_cvt_val ev2)) v).
+Proof using.
+  intros ? ? ? ? ? ? ? ? ? ? ?.
+  subst evalt.
+  unfold cps_cvt_apply.
+  addContVarsSpec 3 Hvc kv.
+  rewrite eval_ret.
+  simpl. unfold subst. 
+  assert (sub_range_sat [(kv, k)] closed) as Hcs by
+    (intros ? ? ?; in_reasoning; cpx).
   rewrite ssubstRet_c by assumption.
   rewrite ssubstKlam_c; [| try assumption| noRepDis].
+  rewrite ssubstRet_c by assumption.
+  rewrite ssubstKlam_c; [| assumption| noRepDis].
+  rewrite ssubstCall_c by assumption.
+  do 3 rewrite ssubst_vterm. simpl.
+  rewrite <- beq_var_refl.
+  do 2 (rewrite not_eq_beq_var_false;[| noRepDis]).
+  unfold isprogram in Hp.
+  rwsimpl Hvc.
+  repnd. unfold closed in *.
+  do 2 (rewrite ssubst_trivial2_cl;[|assumption|];
+          [| unfold closed; symmetry;rewrite cps_cvt_aux_fvars; [| ntwfauto|]; 
+           try rewrite Hp1 ; try rewrite Hp2 ; [ tauto | eauto ] ] ).
+  clear Hcs. rename Hclk into Hclkb.
+  match goal with
+  [|- context [Ret_c _ ?k]] => assert (closed k) as Hclk
+  end.
+    unfold closed. simpl. autorewrite with list core SquiggleEq SquiggleEq2.
+    symmetry.
+    rewrite cps_cvt_aux_fvars;[| ntwfauto|]; try rewrite Hclkb; [  | eauto ].
+    simpl. rewrite Hp1.
+    rewrite remove_nvars_nops;[| noRepDis].
+    autorewrite with SquiggleEq. refl.
+
+  rewrite H1e0; [| assumption]. 
+  simpl. clear H1e0.
+  rewrite cps_val_ret_flip; autounfold with eval; eauto with eval;[].
+  rewrite eval_ret. simpl.
+  unfold subst.
+  rewrite ssubstRet_c by assumption.
+  clear Hclk.
+  rewrite ssubst_trivial2_cl; auto;
+    [ |  (intros ? ? ?; in_reasoning; cpx)| ]; try eauto with eval;[].
+  unfold cps_cvt_val, closed.
+  rewrite ssubstKlam_c; [| (intros ? ? ?; in_reasoning; cpx);
+    apply cps_cvt_val_closed; eauto with eval | noRepDis].
   rewrite ssubstCall_c by assumption.
   do 2 rewrite ssubst_vterm. simpl.
   rewrite <- beq_var_refl.
   rewrite not_eq_beq_var_false;[| noRepDis].
-  rewrite ssubst_trivial2_cl;[| assumption | 
-      symmetry; rewrite cps_cvt_aux_fvars; [ rwHyps; refl | ntwfauto| tauto]].
-  rewrite ssubst_trivial2_cl;[| assumption | assumption].
-  clear Hcs.
-  rename Hclk into Hclkb.
+  rewrite ssubst_trivial2_cl;
+    [| (intros ? ? ?; in_reasoning; cpx); eauto with eval | assumption].
   match goal with
-  [|- context [Ret_c _ ?k]] => assert (closed k) as Hclk;
-    [|  assert (sub_range_sat [(fresh_var [] , k)] closed) as Hcs by
-        (intros ? ? ?; in_reasoning; cpx)]
+  [|- context [Ret_c _ ?k]] => assert (closed k) as Hclk
   end.
-    unfold closed.
-    match type of Hclkb with
-    closed ?k => remember k as kr
-    end.
-    
-    simpl.
-    autorewrite with list core SquiggleEq using rwHyps. refl.
-    rwHyps. rwsimplC. autorewrite with list core SquiggleEq.
-  clear Hcs.
-  rewrite IHHe2 by assumption. clear IHHe2.
-  rewrite cps_val_ret_flip; auto;[|eauto using eval_yields_value'| tauto | split; auto; 
-      eauto using eval_preseves_wf].
+    unfold closed. symmetry.
+    simpl. rewrite Hclkb. rwsimplC.
+    rewrite cps_cvt_val_fvars; eauto with eval.
+    rewrite eval_preserves_closed; eauto. simpl. rwsimplC. refl.
+  rewrite H2e0 by assumption. clear H2e0.
+  rewrite cps_val_ret_flip; eauto with eval.
   rewrite eval_ret.
   simpl. unfold subst.
   rewrite ssubstCall_c by assumption.
   rewrite ssubst_vterm. simpl ssubst_aux.
   rewrite <- beq_var_refl.
-  pose proof Hcle as Hcleb.
-  apply cps_cvt_val_closed in Hcle; eauto using eval_preseves_wf; try tauto.
-  unfold closed in Hcle.
-  do 2 (rewrite ssubst_trivial2_cl;[|intros; repeat in_reasoning; cpx | 
-    assumption
-      ]).
-  rewrite eval_call.
-  rewrite ssubstRet_c. repnd.
-  rewrite <- ssubst_sub_filter2 with (l:=[contVar]).
-  Focus 3. 
-    rewrite cps_cvt_aux_fvars;
-       [disjoint_reasoningv2
-         |(apply' eval_preseves_wf He1; 
-                      ntwfauto) 
-        | assumption]; fail.
-
-  Focus 2. unfold disjoint_bv_sub. unfold cps_cvt_val.
-     intros ? ? Hin. 
-     repeat in_reasoning; inverts Hin;
-     rwHyps; auto.
-     
-  rewrite ssubst_vterm. simpl.
-  autorewrite with SquiggleEq.
-  rewrite not_eq_beq_var_false;[| apply disjoint_neq; disjoint_reasoningv2].
-  rewrite <- (eval_c_ssubst_commute);[refl
-     | apply' eval_preseves_wf He1; 
-                      ntwfauto; eauto using eval_preseves_wf
-     | | | | rwsimplC; try tauto ]; 
-    intros ? ? Hin; rewrite in_single_iff in Hin;
-    inverts Hin; subst;auto;
-        [eapply eval_yields_value'; eauto
-        | ntwfauto; eauto using eval_preseves_wf].
+  do 2 (rewrite ssubst_trivial2_cl;[|intros; repeat in_reasoning; cpx |]; eauto with eval).
+  refl.
 Qed.
+
 
 
 Lemma eval_vals_r:   forall es vs
@@ -2205,17 +2367,6 @@ Proof using.
     autorewrite with list; auto.
 - rewrite <- combine_map_snd;
   autorewrite with list in *; auto.
-Qed.
-
-Lemma eval_proj :
-  forall (lbt : list CBTerm) (i : nat) (k v' : CTerm) (xf: NVar) (fn : CTerm) len,
-    select i lbt = Some (bterm [xf] fn) ->
-    len = length lbt ->
-  let Fix := coterm (CFix len) lbt in
-  eval_c (Proj_c Fix i k) v' <-> eval_c (Ret_c (fn {xf := Fix}) k) v'.
-Proof using.
-  intros ?  ? ? ? ? ? ? Hf Hl; simpl; subst; split ; intros;[| econstructor; eauto].
-  inverts H. simpl in *. unfold Fix_c', subst in *. congruence. 
 Qed.
 
 
@@ -2407,6 +2558,30 @@ Proof using.
 Qed.
 
 
+Lemma eval_FixApp :
+forall (lbt : list CBTerm) (i : nat) (k arg v : CTerm) (bt : CBTerm) l,
+  let len := Datatypes.length lbt in
+  let pinds := seq 0 len in
+  let sub := map (Fix_c' lbt) pinds in
+  select i lbt = Some bt ->
+  l = length lbt ->
+  let Fix := coterm (CFix l i) lbt in
+  eval_c (Call_c Fix k arg) v <->
+  eval_c (Call_c (apply_bterm bt sub) k arg) v.
+Proof using.
+  intros ?  ? ? ? ? ? ? ? ? ? ? ?; simpl; subst; split ; intros;[| econstructor; eauto].
+  inversion H0. subst. clear H0.
+  rewrite H7 in H. inverts H.
+  exact H8.
+Qed.
+
+
+
+
+
+
+
+Local Transparent ssubst.
 Ltac unfoldSubst :=
   unfold ssubst; simpl;
   fold (@ssubst NVar _ _ _ L5Opid);
@@ -2414,12 +2589,397 @@ Ltac unfoldSubst :=
   fold (@ssubst NVar _ _ _ L4Opid);
   fold (@ssubst_bterm NVar _ _ _ L4Opid).
 
-(** What happens when e does not compute further, e.g. eval e e ? 
-Should we prove something more about such cases, e.g. the CPS converted term
-does not admit any evaluations in the user space?*)
+Lemma cps_cvt_corr_app_let_common_part:
+forall x el v2 k v
+(Hp :  isprogram v2)
+(Hv :  is_value v2)
+(Hwf : nt_wf  el)
+(Hfwf : fixwf el = true)
+(Hclk : closed k)
+(Hvc : varsOfClass (all_vars el++ all_vars v2 ++ [x]) USERVAR),
+eval_c (Call_c (cps_cvt_lambda cps_cvt x el) k (cps_cvt_val v2)) v <->
+eval_c (Ret_c (cps_cvt (ssubst el [(x, v2)])) k) v.
+Proof using.
+  intros. unfold isprogram,  closed, closed_bt in *. repnd.
+  pose proof Hvc as Hdis.
+  apply userVarsContVar in Hdis.
+  rwsimpl Hvc. simpl in *.
+  unfold  val_outer, cps_cvt_lambda.
+  rewrite eval_call.
+  rewrite ssubstRet_c. repnd.
+  rewrite <- ssubst_sub_filter2 with (l:=[contVar]).
+  Focus 3. 
+    rewrite cps_cvt_aux_fvars;
+       [disjoint_reasoningv2
+         | ntwfauto
+         | assumption]; fail.
+
+  Focus 2. unfold disjoint_bv_sub. unfold cps_cvt_val.
+     intros ? ? Hin. 
+     repeat in_reasoning; inverts Hin;
+     rwHyps; auto.
+     rewrite cps_cvt_val_fvars; eauto.
+     rwHyps. disjoint_reasoningv.
+     
+  rewrite ssubst_vterm. simpl.
+  autorewrite with SquiggleEq.
+  rewrite not_eq_beq_var_false;[| apply disjoint_neq; disjoint_reasoningv2].
+  rewrite <- (eval_c_ssubst_commute); auto; [
+    
+                      ntwfauto; eauto using eval_preseves_wf
+     | | |  | rwsimplC; try tauto ]; 
+    intros ? ? Hin; rewrite in_single_iff in Hin;
+    inverts Hin; subst;eauto.
+Qed.
+
+Lemma cps_cvt_val_ssubst_commute :
+      forall (e : NTerm) (sub : Substitution),
+       nt_wf e ->
+       fixwf e = true ->
+       is_valueb e = true ->
+       sub_range_sat sub is_value ->
+       sub_range_sat sub nt_wf ->
+       sub_range_sat sub closed ->
+       varsOfClass (all_vars e ++ dom_sub sub ++ flat_map all_vars (range sub)) true ->
+       let sub_c := map_sub_range (cps_cvt_val' cps_cvt) sub in
+       ssubst (cps_cvt_val e) sub_c = cps_cvt_val (ssubst e sub).
+Proof using.
+  intros ? ? Hfwf Hval. intros.
+  change_to_ssubst_aux8.
+-  apply cps_cvt_val_ssubst_commutes_aux; auto. intros.
+  apply eval_c_ssubst_aux_commute; auto.
+(* the rest of this proof was copied exactly from [eval_c_ssubst_commute] *)
+- subst sub_c.
+  rewrite disjoint_flat_map_r.
+  setoid_rewrite map_map.
+  autorewrite with SquiggleEq in H3. repnd.
+  intros t Hin.
+  apply in_map_iff in Hin.
+  exrepnd.
+  specialize (H0 _ _ Hin0).
+  specialize (H1 _ _ Hin0).
+  specialize (H2 _ _ Hin0).
+  simpl in *.
+  apply (f_equal free_vars) in Hin1.
+  rewrite <- Hin1.
+  apply in_sub_eta in Hin0. repnd.
+  eapply varsOfClassSubset in H3;[| eapply subset_flat_map_r; eauto].
+  rewrite cps_cvt_val_fvars; auto.
+  rewrite H2.
+  auto.
+Qed.
+
+Lemma evalt_eval_refl : forall v,
+  eval v v-> evalt v v.
+Proof using.
+  intros. unfold evalt. tauto.
+Qed.
+
+
+
+Lemma eq_iff : forall A B:Prop,
+  A=B -> A <-> B.
+Proof using. intros. subst. refl.
+Qed.
+
+
+Lemma is_lambdab_ssubst_aux : forall nt s,
+  is_lambdab nt = true -> is_lambdab (ssubst_aux nt s) = true.
+Proof using.
+  intros ? ? Hl.
+  destruct nt as [? | o ? ]; inverts Hl as Hl.
+  destruct o; inverts Hl.
+  refl.
+Qed.
+
+Lemma fixwf_ssubst_aux : forall  a sub,
+  sub_range_sat sub (fun x => fixwf x = true)
+  -> fixwf a= true -> fixwf (ssubst_aux a sub) = true.
+Proof using.
+  intros t. induction t as [v | o lbt Hind] using NTerm_better_ind; intros ? Hsr Hwf.
+- simpl. dsub_find sf;[| refl]; symmetry in Heqsf.
+  apply sub_find_some in Heqsf. apply Hsr in Heqsf. auto.
+- rewrite <- Hwf. simpl. f_equal;[ destruct o; try refl;[] | ];
+   rewrite map_map;
+   f_equal;
+   apply eq_maps;
+   intros bt Hin;
+   destruct bt as [lv nt];
+   unfold compose in *;
+   simpl in Hwf;
+    (try (apply andb_true_iff in Hwf; repnd));
+  try(
+   rewrite ball_map_true in Hwf; unfold compose in *;
+   specialize (Hwf _ Hin);
+   simpl in *;
+   rewrite Hwf;
+   eapply Hind; eauto
+   ).
+   rewrite ball_map_true in Hwf0; unfold compose in *;
+   specialize (Hwf0 _ Hin);
+   simpl in *;
+   rewrite Hwf0.
+   apply is_lambdab_ssubst_aux; auto.
+Qed.
+
+(* Move to [SquiggleEq] *)
+Lemma getopid_ssubst_aux_var_ren : forall (a : NTerm) sub,
+   allvars_sub sub
+  -> getOpid (ssubst_aux a sub) = getOpid a.
+Proof using vartype.
+  intros nt sub H.
+  destruct nt; auto.
+   apply isvarc_ssubst_vterm with (v:=n) in H.
+    simpl in *. unfold isvarc in H. dsub_find sc; auto.
+    destruct scs; auto. contradiction.
+Qed.
+
+Lemma fixwf_ssubst_aux_var_ren : forall  a sub,
+   allvars_sub sub
+  -> fixwf (ssubst_aux a sub) = fixwf a.
+Proof using vartype.
+  intros t. induction t as [v | o lbt Hind] using NTerm_better_ind; intros ? ?.
+- apply isvarc_ssubst_vterm with (v0:=v) in H.
+  simpl in *. unfold isvarc in H. dsub_find sc; auto.
+  destruct scs; auto.
+-  simpl. f_equal;[ destruct o; try refl;[] | ];
+   rewrite map_map;
+   f_equal;
+   apply eq_maps;
+   intros bt Hin;
+   destruct bt as [lv nt];
+   unfold compose in *; simpl in *;
+   try (eapply Hind; eauto using sub_filter_allvars);[].
+    unfold is_lambdab. rewrite getopid_ssubst_aux_var_ren.
+   refl.
+   apply sub_filter_allvars. auto.
+Qed.
+
+
+(* Move to [SquiggleEq] 
+Lemma ssubst_aux_var_ren_impl_alpha {A:Type} : 
+  forall (f: NTerm -> A),
+   (forall a sub, allvars_sub sub -> f (ssubst_aux a sub) = f a)
+ -> forall (a b: NTerm), alpha_eq a b -> f a = f b.
+Proof using.
+  intros  ?  H ?.
+  nterm_ind1s a as [? | o lbt Hind] Case; intros ? Hal; inverts Hal; auto.
+  simpl.
+
+
+ f_equal; [
+    destruct o; auto |].
+*)
+  
+
+Global Instance fixwf_alpha :
+  Proper (alpha_eq  ==> eq) fixwf.
+Proof using.
+  intros a b H. apply alpha_eq3_if with (lv:=[]) in H.
+  revert H. revert b. revert  a.
+  nterm_ind1s a as [? | o lbt Hind] Case; intros ? Hal;
+   inverts Hal; auto.
+  simpl. f_equal; [
+    destruct o; auto |]; f_equal;
+  unfold compose;
+  apply eq_maps_bt; auto;
+  intros ? Hlt;
+  specialize (H3 _ Hlt);
+  pose proof Hlt as Hlt1;
+  pose proof Hlt as Hlt2;
+  rewrite H1 in Hlt2;
+  pose proof (selectbt_in _ _ Hlt1);
+  pose proof (selectbt_in _ _ Hlt2);
+  destruct (selectbt lbt n) as [lv1 nt1];
+  destruct (selectbt lbt2 n) as [lv2 nt2]; simpl;
+  inverts H3 as ? ? ? ? Hal.
++ unfold is_lambdab. apply alpha_eq_if3 in Hal.
+  apply alphaGetOpid in Hal.
+  do 2 rewrite getopid_ssubst_aux_var_ren in Hal 
+    by (eauto 1 using allvars_combine).
+  rewrite Hal. refl.
++ eapply Hind in Hal; eauto;
+  try rewrite ssubst_aux_allvars_preserves_size2; try omega.
+  do 2 (rewrite  fixwf_ssubst_aux_var_ren in Hal 
+    by (eauto 1 using allvars_combine)).
+  assumption.
+Qed.
+
+(* this lemma is the crux of [eval_preserves_fixwf] below *)
+Lemma fixwf_ssubst : forall  a sub,
+  sub_range_sat sub (fun x => fixwf x = true)
+  -> fixwf a= true -> fixwf (ssubst a sub) = true.
+Proof using.
+  intros ? ? ? Hwf.
+  rewrite ssubst_ssubst_aux_alpha.
+  add_changebvar_spec nt' XX.
+  repnd. rewrite XX in Hwf.
+  eapply fixwf_ssubst_aux; auto.
+Qed.
+
+Lemma eval_preserves_fixwf :
+  forall e v, eval e v ->  fixwf e = true -> fixwf v = true.
+Proof using.
+  intros ? ? He. induction He; intro Hfwf; try auto.
+- apply_clear IHHe3. 
+  simpl in *. repeat rewrite andb_true_iff in *.
+  unfold compose in *. simpl in *. repnd.
+  apply fixwf_ssubst; [| tauto].
+  prove_sub_range_sat.
+
+- revert Hfwf.
+  simpl.
+  repeat rewrite map_map.
+  unfold compose.
+  rewrite (combine_map_snd es vs) by assumption.
+  setoid_rewrite (combine_map_fst es vs) at 1;[|assumption].
+  repeat rewrite map_map.
+  repeat rewrite ball_map_true in *. simpl.
+  intro Hfwf. firstorder.
+
+- apply_clear IHHe2. (* this is same as the app(1st) case with IHHe2 instead of IHHe3 *)
+  simpl in *. repeat rewrite andb_true_iff in *.
+  unfold compose in *. simpl in *. repnd.
+  apply fixwf_ssubst; [| tauto].
+  prove_sub_range_sat.
+
+- apply_clear IHHe2. destruct e'.
+  simpl in *. repeat rewrite andb_true_iff in *.
+  unfold compose in *. simpl in *. repnd.
+  repeat rewrite map_map in *.
+  repeat rewrite ball_map_true in *. simpl in *.
+  unfold apply_bterm. simpl.
+  apply find_branch_some in H. repnd.
+  specialize (Hfwf _ H0). simpl in *.
+  apply fixwf_ssubst; auto.
+  intros ? ? Hin. apply IHHe1; auto.
+  apply in_combine_r in Hin. assumption.
+
+- apply_clear IHHe3. destruct bt. 
+  simpl in *. repeat rewrite andb_true_iff in *.
+  unfold compose in *. simpl in *. repnd.
+  dands; eauto 2. GC.
+  apply fixwf_ssubst; auto 1.
+  + unfold sub. intros ? ? Hin.
+    apply in_combine in Hin. repnd.
+    apply in_map_iff in Hin.
+    exrepnd. subst. simpl. auto.
+    repeat rewrite andb_true_iff. auto.
+  + apply select_in in H.
+    repeat rewrite ball_map_true in *.
+    specialize (IHHe1 Hfwf0). repnd.
+    specialize (IHHe1 _ H). simpl in *.
+    auto.
+Qed.
+
+
+Hint Resolve eval_preserves_fixwf : eval.
+Ltac ntwfautoFast :=
+unfold apply_bterm in *;
+unfold subst in *;
+(repeat match goal with
+| [ H: nt_wf ?x |- _ ] => 
+  let H1 := fresh "Hntwf" in
+  let H2 := fresh "HntwfSig" in
+    inverts H as H1 H2;[]; simpl in H1; dLin_hyp
+| [ H: _ -> (nt_wf _) , H1:_ |- _ ] => apply H in H1; clear H
+| [ H: forall (_:_),  _ -> (nt_wf _) , H1:_ |- _ ] => apply H in H1
+| [ H: forall (_:_),  _ -> (bt_wf _) , H1:_ |- _ ] => apply H in H1
+| [ H: bt_wf (bterm _ _) |- _ ] => apply bt_wf_iff in H
+| [ |- nt_wf (vterm _)] => constructor
+| [ |- bt_wf _] => constructor
+| [ H: _ \/ False |- _] => rewrite or_false_r in H; subst
+| [ |- nt_wf _] => 
+  let Hin := fresh "HntwfIn" in
+    constructor; [try (intros ? Hin; simpl in Hin; in_reasoning; subst;  cpx)|]
+end); cpx.
+
+
+(* Move to SquiggleEq *)
+Lemma map0lbt : forall (lbt: list BTerm),
+map num_bvars lbt = repeat 0 (Datatypes.length lbt)
+->  lbt = map (bterm []) (map get_nt lbt).
+Proof using.
+  induction lbt; simpl; auto.
+  intro Hn.
+  destruct a. inverts Hn as Hn Hnn. unfold num_bvars in Hn.
+  simpl in Hn. dlist_len_name l Hh.
+  simpl. f_equal. eauto.
+Qed.
+
+Lemma is_valueb_sound :
+  (forall e,  is_valueb e = true -> nt_wf e-> is_value e).
+Proof using.
+  intros ? Hisv Hnt.
+  nterm_ind e as [? | o lbt Hind] Case; [constructor|].
+  inverts Hnt as Hbt Hnb.
+  destruct o ; simpl in Hnb; try inverts Hisv.
+- dnumvbars Hnb l. constructor. 
+- apply (f_equal (@length _ )) in Hnb. 
+  rewrite map_length, repeat_length in Hnb. subst.
+  constructor.
+- pose proof Hnb as Hnbb. 
+  apply (f_equal (@length _ )) in Hnb. 
+  rewrite map_length, repeat_length in Hnb. subst.
+  apply map0lbt in Hnbb.
+  rewrite Hnbb. do 1 rewrite map_length.
+  apply con_is_value.
+  rewrite ball_map_true in H0.
+  intros ? Hin.
+  apply in_map with (f:=(bterm [])) in Hin.
+  pose proof Hin as Hinb.
+  rewrite <- Hnbb in Hin.
+  apply H0 in Hin. unfold compose in Hin. simpl in Hin.
+  rewrite <- Hnbb in Hinb.
+  apply Hind with (lv:=[]); eauto.
+  ntwfauto.
+Qed.
+
+Lemma is_value_eval_end : forall v,
+  is_value v 
+  -> closed v
+  -> eval v v.
+Proof using.
+  intros ? Hv.
+  induction Hv; try econstructor; auto.
+- intro c. inverts c.
+- intros ? ? Hin.
+  rewrite <- (map_id es) in Hin.
+  rewrite combine_map in Hin.
+  apply in_map_iff in Hin.
+  exrepnd. inverts Hin1.
+  apply H0; auto.
+  unfold closed in *.
+  simpl in H1.
+  rewrite flat_map_map in H1.
+  rewrite flat_map_empty in H1.
+  apply H1 in Hin0.
+  auto.
+Qed.
+
+
+Lemma eval_end : forall e v,
+  eval e v -> eval v v.
+Proof using.
+  intros ? ? Hev.
+  induction Hev; auto; try constructor; try auto.
+  intros ? ? Hin.
+  rewrite <- (map_id vs) in Hin.
+  rewrite combine_map in Hin.
+  apply in_map_iff in Hin.
+  exrepnd.
+  inverts Hin1.
+  apply combine_in_right with (l1:=es) in Hin0;[| omega].
+  exrepnd.
+  eapply H1; eauto.
+Qed.
+
+Hint Resolve eval_end : eval.
+
 
 Theorem cps_cvt_corr : forall e v,
   nt_wf e ->
+  fixwf e = true ->
   varsOfClass (all_vars e) USERVAR -> 
   eval e v ->
   closed e ->
@@ -2428,86 +2988,43 @@ Theorem cps_cvt_corr : forall e v,
       eval_c (Ret_c (cps_cvt e) k) v' <->
         eval_c (Ret_c (cps_cvt v) k) v'.
 Proof using.
-  intros ? ? Hwf Hvc He.  induction He; try (simpl ; tauto; fail); [ | | | |]. 
+  intros ? ? Hwf Hfwf Hvc He.  induction He; try (simpl ; tauto; fail); [ | | | |].
   (* beta reduction case (eval_App_e) *)
-- intros Hcle ? Hcl ?.
-   unfold App_e in *. simpl.
-   unfold cps_cvt_apply.
+- intros Hcle ? Hcl ?. simpl.
+  unfold App_e in *. simpl.
   repeat progress (autorewrite with list allvarsSimpl in Hvc; 
     simpl in Hvc).
-  addContVarsSpec 3 Hvc kv.
-  simpl.
-  repnd.
-  (* now lets fulfil the assumptions in the induction hypotheses *)
   unfold closed in Hcle. simpl in Hcle.
-  autorewrite with core list in Hcle.
+  rwsimpl Hcle.
   apply app_eq_nil in Hcle.
-  autorewrite with SquiggleEq in *. repnd.
-  pose proof He1 as He1wf.
+  progress autorewrite with SquiggleEq in *. repnd.
+  ntwfauto.
+  simpl in Hfwf. repeat rewrite andb_true_iff in Hfwf. unfold compose in Hfwf.
+  simpl in Hfwf. repnd.
+  rewrite cps_cvt_apply_eval; unfold evalt; unfold isprogram; dands; eauto;
+    [| rwsimplC; tauto ].
+  clear IHHe1 IHHe2.
+  pose proof He1 as He1wf.  
   apply' eval_preseves_wf He1wf.
-  dimp He1wf;clear He1wf;[ ntwfauto|]. rename hyp into He1wf.
-  specialize (IHHe1 ltac:(ntwfauto) Hvc0  Hcle0).
-  specialize (IHHe2 ltac:(ntwfauto) Hvc Hcle).
-  specialize (IHHe3 ltac:(ntwfauto; eauto using eval_preseves_wf)).
-  (* IHHe3 needs more work : 2 more hyps *)
   applydup (eval_preseves_varclass USERVAR) in He1 as Hvs1;[| assumption].
-  applydup (eval_preseves_varclass USERVAR) in He2 as Hvs2;[| assumption].
   unfold Lam_e in Hvs1.
   rwsimpl Hvs1. repnd.
-  dest_imp IHHe3 HH;[apply ssubst_allvars_varclass_nb;  rwsimplC; try tauto|].
-
-  (* IHHe3 has 1 more hyp *)
   applydup eval_preserves_closed in He1 as Hss;[| assumption].
   applydup eval_preserves_closed in He2 as Hss2;[| assumption].
   unfold subst, closed in *. simpl in *. autorewrite with list in *.
-  setoid_rewrite fvars_ssubst1 in IHHe3;[| intros; repeat in_reasoning; cpx].
-  dest_imp IHHe3 HH.
-
-  rewrite <- IHHe3;[| assumption]. clear IHHe3.
-
-  (* now, work on simplifying LHS slowly until it becomes equal to rhs *)
-  (* first, e1 will be evaluated to a lambda *) 
-  rewrite eval_ret.
-  simpl. unfold subst. 
-  assert (sub_range_sat [(kv, k)] closed) as Hcs by
-    (intros ? ? ?; in_reasoning; cpx).
-  rewrite ssubstRet_c by assumption.
-  rewrite ssubstKlam_c; [| try assumption| noRepDis].
-  rewrite ssubstRet_c by assumption.
-  rewrite ssubstKlam_c; [| assumption| noRepDis].
-  rewrite ssubstCall_c by assumption.
-  do 3 rewrite ssubst_vterm. simpl.
-  rewrite <- beq_var_refl.
-  do 2 (rewrite not_eq_beq_var_false;[| noRepDis]).
-  do 2 (rewrite ssubst_trivial2_cl;[|assumption|];
-          [| unfold closed; symmetry;rewrite cps_cvt_aux_fvars; [| ntwfauto|]; 
-           try rewrite Hcle0 ; try rewrite Hcle ; [ tauto | eauto ] ] ).
-
-  clear Hcs.
-  match goal with
-  [|- context [Ret_c _ ?k]] => assert (closed k) as Hclk
-  end.
-    unfold closed. simpl. autorewrite with list core SquiggleEq SquiggleEq2.
-    symmetry.
-    rewrite cps_cvt_aux_fvars;[| ntwfauto|]; try rewrite Hcle; [  | eauto ].
-    simpl. rewrite Hcl.
-    rewrite remove_nvars_nops;[| noRepDis].
-    autorewrite with SquiggleEq. refl.
-
-  rewrite IHHe1; [| assumption]. 
-  simpl. clear IHHe1.
-  eapply cps_cvt_corr_app_let_common_part; unfold isprogram, isprogram_bt; dands; eauto;
-    rwsimplC; try tauto; try ntwfauto.
-
-  apply userVarsContVar in Hvc.
-  applydup userVarsContVar in Hvs1.
-  applydup userVarsContVar in Hvs0.
-  apply userVarsContVars with (n:=3) in Hvs1.
-  apply userVarsContVars with (n:=3) in Hvs0.
-  rewrite <- Heqlvcvf in Hvs0, Hvs1.
-  rewrite cons_as_app.
-  remember ([kv, kv0, kv1]) as cv. clear Heqcv Heqlvcvf.
-  noRepDis.
+  pose proof (eval_preserves_fixwf _ _ He1 Hfwf0) as Hfwflam.
+  pose proof (eval_preserves_fixwf _ _ He2 Hfwf1) as Hfwfarg.
+  simpl in Hfwflam. unfold compose in Hfwflam. simpl in Hfwflam.
+  rewrite andb_true_r in Hfwflam.
+  rewrite <- IHHe3; eauto with eval;
+    [ | ntwfauto; eauto with eval 
+      | apply fixwf_ssubst; auto; prove_sub_range_sat; auto
+      | apply ssubst_allvars_varclass_nb; rwsimplC; dands; eauto with eval
+      | setoid_rewrite fvars_ssubst1;[assumption | intros; repeat in_reasoning; cpx]].
+  clear IHHe3.
+  rewrite cps_cvt_corr_app_let_common_part; eauto with eval; 
+    [refl | ntwfauto   |].
+  rwsimplC; dands; eauto with eval.
 
 (* reduction inside constructor : eval_Con_e *)
 - intros Hcle ? Hcl ?. rename H0 into Hev. rename H1 into Hind.
@@ -2554,74 +3071,52 @@ Proof using.
   intros ? ? Hinn.
   applydup in_combine_l in Hinn.
   rewrite flat_map_empty in Hcle.
-  apply Hind; auto;[].
-  eapply varsOfClassSubset;[| apply Hvc].
-  apply subset_flat_map_r. auto.
+  rewrite map_map in Hfwf. rewrite ball_map_true in Hfwf.
+  unfold compose in Hfwf.
+  specialize (Hfwf _ Hinn0). simpl in Hfwf.
+  apply Hind; auto;[ ].
+  eauto with subset.
 
 (* eval_Let_e *)
-- intros Hcle ? Hcl ?.
-   unfold Let_e in *. simpl.
-   unfold cps_cvt_apply.
+- intros Hcle ? Hcl ?. simpl.
+  unfold Let_e in *. simpl.
+  change
+    (val_outer (cps_cvt_lambda cps_cvt x e2))
+    with (cps_cvt (Lam_e x e2)).
+  unfold Lam_e in *.
   repeat progress (autorewrite with list allvarsSimpl in Hvc; 
     simpl in Hvc).
-  addContVarsSpec 3 Hvc kv.
-  simpl.
-  repnd.
-  (* now lets fulfil the assumptions in the induction hypotheses *)
   unfold closed in Hcle. simpl in Hcle.
-  autorewrite with core list in Hcle.
+  rwsimpl Hcle.
   apply app_eq_nil in Hcle.
-  applydup userVarsContVar in Hvc as Hvcdiss.
-  autorewrite with SquiggleEq in *. repnd.
-  specialize (IHHe1 ltac:(ntwfauto) Hvc0  Hcle0).
-  specialize (IHHe2 ltac:(apply' eval_preseves_wf He1; 
-                      ntwfauto; eauto using eval_preseves_wf)).
-  (* IHHe3 needs more work : 2 more hyps *)
-  applydup (eval_preseves_varclass USERVAR) in He1 as Hvs1;[| assumption].
-  rewrite cons_as_app in Hvc.
-  rwsimpl Hvc.
-  dest_imp IHHe2 HH;[apply ssubst_allvars_varclass_nb;  rwsimplC; tauto|].
+  progress autorewrite with SquiggleEq in *. repnd.
+  ntwfauto. rewrite cons_as_app in Hvc. rwsimpl Hvc. repnd.
+  simpl in Hfwf.
+  unfold compose in Hfwf. simpl in Hfwf.
+  rewrite andb_true_r in Hfwf.
+  repeat rewrite andb_true_iff in Hfwf. repnd.
+  pose proof (eval_preserves_fixwf _ _ He1 Hfwf0) as Hfwflam.
 
-  rename e2 into e1'.
-  rename IHHe2 into IHHe3.
-  applydup eval_preserves_closed in He1 as Hss;[| assumption].
-  unfold subst, closed in *. simpl in *. autorewrite with list in *.
-  setoid_rewrite fvars_ssubst1 in IHHe3;[| intros; repeat in_reasoning; cpx].
-  dest_imp IHHe3 HH.
+  rewrite cps_cvt_apply_eval; unfold evalt; unfold isprogram, closed; dands;
+    eauto using eval_Lam_e; eauto with eval; try tauto;
+    [| rwsimplC; auto | ntwfauto | rwsimplC; tauto];[].
 
-  rewrite <- IHHe3;[| assumption]. clear IHHe3.
-  
-  rewrite eval_ret.
-  simpl. unfold subst. 
-  assert (sub_range_sat [(kv, k)] closed) as Hcs by
-    (intros ? ? ?; in_reasoning; cpx).
-  rewrite ssubstRet_c by assumption.
-  rewrite ssubstKlam_c; [| try assumption| noRepDis].
-  rewrite ssubstRet_c by assumption.
-  rewrite ssubstKlam_c; [| assumption| noRepDis].
-  rewrite ssubstCall_c by assumption.
-  do 3 rewrite ssubst_vterm. simpl ssubst_aux.
-  rewrite <- beq_var_refl.
-  do 2 (rewrite not_eq_beq_var_false;[| noRepDis]).
-  change (val_outer (cps_cvt_lambda cps_cvt x e1')) with
-            (cps_cvt (Lam_e x e1')).
-  (rewrite ssubst_trivial2_cl;[|assumption|];
-          [| unfold closed, Lam_e in * ; symmetry;
-               rewrite cps_cvt_aux_fvars; simpl; [lcongruence | ntwfauto| rwsimplAll; tauto] ] ).
-  (rewrite ssubst_trivial2_cl;[|assumption|];
-          [| unfold closed in *; symmetry;rewrite cps_cvt_aux_fvars; [congruence | ntwfauto| tauto]] ).
+  clear IHHe1.
+  rewrite <- IHHe2; eauto with eval; unfold closed;
+    [ | ntwfauto; eauto with eval
+      | apply fixwf_ssubst; auto; prove_sub_range_sat; auto
+      | apply ssubst_allvars_varclass_nb; rwsimplC; dands; eauto with eval
+      | setoid_rewrite fvars_ssubst1;
+          [assumption | intros; repeat in_reasoning; cpx]; eauto with eval ].
 
-  eapply cps_cvt_corr_app_let_common_part; unfold isprogram, isprogram_bt; dands; eauto;
-    rwsimplC; try tauto; try ntwfauto;
-    [rewrite cons_as_app; rewrite disjoint_app_l; split;tauto|].
-  
-  unfold closed. simpl. autorewrite with core list SquiggleEq using rwHyps.
-  symmetry. rewrite cps_cvt_aux_fvars; simpl; auto.
-  rwHyps. simpl. rewrite remove_nvars_app_l. 
-  simpl. autorewrite with SquiggleEq. refl.
+  clear IHHe2.
+  simpl.
+  rewrite cps_cvt_corr_app_let_common_part; eauto with eval;
+    [refl | ].
+  rwsimplC; dands; eauto with eval.
+
 
 (* eval_Match_e *)
-
 - intros Hcle ? Hcl ?.
   unfold Match_e in *.
   remember (Con_e d vs) as con.
@@ -2636,7 +3131,9 @@ Proof using.
   unfold closed in *.
   rwsimpl Hcle.
   apply app_eq_nil in Hcle. repnd.
-  specialize (IHHe1 ltac:(ntwfauto) Hvc0  Hcle0).
+  unfold compose in Hfwf. simpl in Hfwf.
+  apply andb_true_iff in Hfwf. repnd.
+  specialize (IHHe1 ltac:(ntwfauto) ltac:(auto) Hvc0  Hcle0).
   apply find_branch_some in H as H. rename H into Hfr.
 
   unfold num_bvars in Hfr.
@@ -2655,18 +3152,28 @@ Proof using.
   rwsimpl Hcvc.
   unfold Con_e, closed in Hc. simpl in Hc.
   rwsimpl Hc.
+  pose proof (eval_preserves_fixwf _ _ He1 Hfwf0) as Hfwflam.
+  simpl in Hfwflam. 
+  repeat rewrite map_map, ball_map_true in *.
+  specialize (Hfwf _ Hfr0).
   dimp IHHe2.
     apply ssubst_wf_iff;[| auto].
     apply sub_range_sat_range.
     rewrite dom_range_combine by assumption.
     ntwfauto. autorewrite with SquiggleEq in Hntwf. assumption.
-  rename hyp into Hwfs. specialize (IHHe2 Hwfs).
+    rename hyp into Hwfs. specialize (IHHe2 Hwfs).
+
+  dimp IHHe2.
+    apply fixwf_ssubst; auto.
+    simpl. prove_sub_range_sat. apply in_combine_r in Hin.
+    apply Hfwflam. auto.
+    specialize (IHHe2 hyp). clear hyp.
   
   dimp IHHe2.
     apply ssubst_allvars_varclass_nb. simpl.
     rewrite dom_range_combine by assumption.
     rwsimplC. split; eauto with subset.
-  rename hyp into Hvcs. specialize (IHHe2 Hvcs).
+    rename hyp into Hvcs. specialize (IHHe2 Hvcs).
 
   dimp IHHe2.
     apply closed_bt_implies; [ apply Hcleb; assumption 
@@ -2764,74 +3271,134 @@ Proof using.
   + setoid_rewrite <- flat_map_empty. auto.
   + rewrite dom_sub_combine ;[| rwsimplC; auto]. rwsimplC. dands; eauto with subset.
 
-(* eval_Proj_e *)
-- intros Hcle ? Hcl ?. rename He into Hev.
-  ntwfauto. clear HntwfSig.  remember (Lam_e xl bl) as lam.
-  simpl. 
-  Local Opaque cps_cvt cps_cvt_val'.
-  unfold Proj_e, Fix_e', closed in *.
-  simpl in *.
+(* eval_FixApp_e *)
+- intros Hcle ? Hcl ?. simpl.
+  unfold App_e, Fix_e' in *. simpl.
+  repeat progress (autorewrite with list allvarsSimpl in Hvc; 
+    simpl in Hvc).
+  unfold closed in Hcle. simpl in Hcle.
   rwsimpl Hcle.
-  rwsimpl Hvc.
-  applydup eval_preserves_closed in Hev as Hevvc;[| assumption].
-  applydup eval_preseves_wf in Hev as Hevvw;[| assumption].
-  applydup (eval_preseves_varclass USERVAR) in Hev as Hevvvc;[| tauto].
-  applydup cps_cvt_val_closed in Hevvc as Hevcc; [| try assumption |try assumption].
-  apply proj2 in Hvc.
-  addContVarsSpec 2 Hvc kv.
-  unfold closed in *. simpl in *.
-  pose proof Hevvc as Hevvcl.
-  rewrite flat_map_empty in Hevvcl.
+  apply app_eq_nil in Hcle.
+  progress autorewrite with SquiggleEq in *. repnd.
+  ntwfauto.
+  simpl in Hfwf. unfold compose in Hfwf. simpl in Hfwf.
+  rewrite andb_true_r in Hfwf.
+  rewrite andb_true_iff in Hfwf. repnd.
+  rewrite cps_cvt_apply_eval; unfold evalt; unfold isprogram; dands; eauto;
+    [|  rwsimplC; try tauto ].
+  clear IHHe1 IHHe2.
+  pose proof He1 as He1wf.  
+  apply' eval_preseves_wf He1wf.
+  pose proof He2 as He2wf.  
+  apply' eval_preseves_wf He2wf.
+  applydup (eval_preseves_varclass USERVAR) in He1 as Hvs1;[| assumption].
+  unfold Lam_e in Hvs1.
+  rwsimpl Hvs1. repnd.
+  applydup eval_preserves_closed in He1 as Hss;[| assumption].
+  applydup eval_preserves_closed in He2 as Hss2;[| assumption].
+  unfold subst, closed in *. simpl in *. autorewrite with list in *.
+  destruct bt as [lv nt]. simpl in IHHe3.
   pose proof H as Hsel.
   apply select_in in H.
-  specialize (Hevvcl _ H).
-  pose proof Hevvw as  Hevvwb.
-  inverts Hevvw as Hwfes _.
-  specialize (Hwfes _ H). inverts Hwfes.
-  rwsimpl Hevvvc.
+  pose proof (eval_preserves_fixwf _ _ He1 Hfwf0) as Hfwflam.
+  simpl in Hfwflam.
+  specialize (He1wf Hyp).
+
+  pose proof (subset_fvars_fix (bterm lv nt) lbt) as Hssn.
+  simpl in Hssn. rewrite Hss in Hssn.
+  dimp Hssn; auto.
+  clear Hssn. rename hyp into Hssn.
+  apply subsetv_nil_r in Hssn. unfold apply_bterm in Hssn.
+  simpl in Hssn. fold len pinds in Hssn. 
+  unfold Fix_e' in Hssn. fold sub in Hssn.
+
+  clear HntwfSig.
+  let tac t :=
+    prove_sub_range_sat; apply in_combine_r in Hin;
+    unfold sub in Hin;
+    rewrite in_map_iff in Hin;
+    exrepnd; subst; t in
+  assert (sub_range_sat (combine lv sub) (fun x => fixwf x = true))
+    by (tac assumption);
+  assert (sub_range_sat (combine lv sub) is_value)
+    by (tac constructor);
+  assert (sub_range_sat (combine lv sub) nt_wf)
+    by (tac ntwfauto);
+  assert (sub_range_sat (combine lv sub) closed)
+    by (tac auto).
+
+  assert ((varsOfClass (flat_map all_vars (range (combine lv sub)))) true)
+    as Hvcccc.
+    rewrite dom_range_combine; 
+      [| unfold sub, pinds; rewrite map_length, seq_length; auto].
+    pose proof (fVarsFix' lbt) as xxx.
+    unfold Fix_e' in xxx.
+    unfold sub, pinds, len.
+    rewrite xxx. clear xxx. assumption.
   
-  symmetry.
-  match goal with 
-  [|- context [cps_cvt ?x]] => assert (is_value x) as Hisv
-  end.
-    subst. rewrite ssubst_ssubst_aux;[| simpl; rwHyps; simpl; auto].
-    constructor; fail.
-  symmetry.
-  do 1 rewrite eval_ret.
-  simpl. unfold subst.  
-  do 1 rewrite ssubstRet_c.
-  assert (forall x, sub_range_sat [(x, k)] closed) as Hcs by
-    (intros ? ? ? ?; in_reasoning; cpx).
-  rewrite ssubstKlam_c; simpl; auto; [| noRepDis2].
+  assert (varsOfClass (all_vars (ssubst nt (combine lv sub))) true).
+    apply ssubst_allvars_varclass_nb.
+    rwsimplC; dands; eauto with subset.
+
+
+  apply andb_true_iff in Hfwflam.
+  do 2 rewrite ball_map_true in Hfwflam. repnd.
+  specialize (Hfwflam _ H).
+  specialize (Hfwflam0 _ H). 
+  unfold compose in Hfwflam, Hfwflam0. simpl in Hfwflam, Hfwflam0.
+  remember (combine lv sub) as subb.
+
+  assert (varsOfClass (dom_sub subb) true).
+    subst subb. rewrite dom_sub_combine; 
+    [ |unfold sub, pinds; rewrite map_length, seq_length; auto].
+    eauto with subset.
+
+  assert (nt_wf v2) by auto.
+  assert (nt_wf nt) by ntwfauto.
+  assert (nt_wf (ssubst nt subb)) by (apply ssubst_wf_iff; auto).
+  clear Hyp Hyp0 He1wf He2wf.
+  assert (fixwf v2 = true) by (eauto with eval).
+  assert (fixwf (ssubst nt subb) = true) by (apply fixwf_ssubst; auto).
+  unfold sub, pinds in Heqsubb.
+  clear He3. clear sub. clear pinds.
+
+  assert (is_value (ssubst nt subb)).
+    apply is_valueb_sound; auto.
+    change_to_ssubst_aux8.
+    rewrite isvalueb_ssubst_aux; auto.
+    apply is_lambdab_is_valueb; auto.
+
+  rewrite <- IHHe3; rwsimplC; dands; eauto 3 with eval; try eauto 1 with SquiggleEq;
+    [| ntwfautoFast 
+      | unfold compose; simpl; rwHyps; refl | rwHyps; refl ].
+  clear IHHe3.
+
+  unfold cps_cvt_fn_list'.
+  rewrite cps_cvt_apply_eval; try apply evalt_eval_refl; 
+    dands; rwsimplC; eauto with eval;
+    [ | apply is_value_eval_end; auto].
+  
+  rewrite eval_FixApp; rwsimplC; eauto;
+    [ | apply select_map; apply Hsel].
+  apply eq_iff.
+  f_equal.
+  f_equal.
   simpl.
-  rewrite ssubst_trivial2_cl;[ | apply Hcs | apply cps_cvt_closed; auto].
-  unfold Proj_c.
-  unfold ssubst at 1. simpl. 
-  do 1 rewrite <- beq_var_refl.
-  do 1 (rewrite not_eq_beq_var_false;[| noRepDis]).
-  rewrite IHHe; auto;[| rwsimplC; rwHyps; auto].
-  let tac :=auto;unfold Con_e; unfold isprogram, closed; rwsimplC; rwHyps; auto in
-    rewrite cps_val_ret_flip; [|  eauto using eval_yields_value'| tac | tac | tac].
-  prepareForEvalRet Hclkk Hcsss;
-    [apply cps_cvt_val_closed; auto; rwsimplC; auto|].
-  rewrite eval_ret. simpl. unfold subst.
-  unfoldSubst. rewrite <- beq_var_refl.
-  rewrite ssubst_trivial2_cl by assumption.
-  setoid_rewrite eval_proj; try setoid_rewrite map_length; auto;[|].
-  Focus 2.
-    unfold cps_cvt_fn_list'. erewrite select_map;[| apply Hsel]. simpl. refl.
-  simpl. unfold subst.
-  match goal with
-  [|- context [ (_,?ft)]  ] => 
-    change ft with (cps_cvt_val (oterm (NFix (Datatypes.length es)) es))
-  end.
-  apply eq_subrelation;[auto with typeclass_instances|].
-  do 2 f_equal.
-  apply select_in in Hsel.
-  rewrite <- eval_c_ssubst_commute; auto;
-  try complete (prove_sub_range_sat; auto; constructor).
-  rwsimplC. dands; eauto with subset.
+  unfold apply_bterm. simpl.
+  fold len.
+
+  rewrite <- cps_cvt_val_ssubst_commute; eauto using is_lambdab_is_valueb;
+    [| rwsimplC; dands; eauto with subset].
+  f_equal. subst subb.
+  rewrite map_sub_range_combine.
+  f_equal.
+  rewrite map_map.
+  apply eq_maps.
+  intros. simpl.
+  unfold Fix_c'.
+  rewrite map_length. refl.
 Qed.
+(*
 
 (** 
 ** Evaluation of CPS converted terms respects alpha equality. *
@@ -3182,7 +3749,7 @@ Abort.
   
 End TypePreservingCPS.
 
-
+*)
 End VarsOf2Class.
 
 Ltac addContVarsSpec  m H vn:=
