certicoq/theories/allInstances.v
@@ -1,7 +1,7 @@
 Require Export Common.certiClasses.
 Require Export L2.instances.
 Require Export L4.instances.
-Require Export L6.instances.
+(*Require Export L6.instances.*)
 
 
 Quote Recursively Definition p := (3 + 4).
@@ -17,14 +17,17 @@ Print Instances CerticoqLanguage.
 Require Import Common.Common.
 Eval compute in (translateTo (cTerm certiL4) p).
 
-Time Eval compute in (translateTo (cTerm certiL4a) p).
+Time Eval compute in (translateTo (cTerm certiL5a) p).
 
 (* Fix the type of [certiL5a_t0_L6]. It should return (cTerm certiL6) which 
 also contains an environment. 
 To debug typeclass resolution problems, try:
 Typeclasses eauto := 5. (* or a small number to limit the search depth *)
 Typeclasses eauto := debug. (* if your ide doesn't show debug messages, use coqc *)
-*)
+
 Eval vm_compute in (translateTo (* (cTerm certiL6) *) cps.exp p).
+
+
+*)
 
 
